adapt Earley_Set.thy

Earley_Set.thy
@@ -82,17 +82,14 @@ lemma slice_shift:
 
 section \<open>Additional Derivation Lemmas\<close>
 
-context CFG
-begin
-
 lemma Derives1_prepend:
-  assumes "Derives1 u i r v"
-  shows "Derives1 (w@u) (i + length w) r (w@v)"
+  assumes "Derives1 cfg u i r v"
+  shows "Derives1 cfg (w@u) (i + length w) r (w@v)"
 proof -
   obtain x y N \<alpha> where *:
     "u = x @ [N] @ y" "v = x @ \<alpha> @ y"
-    "(N, \<alpha>) \<in> set \<RR>" "r = (N, \<alpha>)" "i = length x"
-    using assms Derives1_def by blast
+    "(N, \<alpha>) \<in> set (\<RR> cfg)" "r = (N, \<alpha>)" "i = length x"
+    using assms Derives1_def by (smt (verit))
   hence "w@u = w @ x @ [N] @ y" "w@v = w @ x @ \<alpha> @ y"
     by auto
   thus ?thesis
@@ -103,17 +100,17 @@ proof -
 qed
 
 lemma Derivation_prepend:
-  "Derivation b D b' \<Longrightarrow> Derivation (a@b) (map (\<lambda>(i, r). (i + length a, r)) D) (a@b')"
-  using Derives1_prepend by (induction D arbitrary: b b') (auto, blast)
+  "Derivation cfg b D b' \<Longrightarrow> Derivation cfg (a@b) (map (\<lambda>(i, r). (i + length a, r)) D) (a@b')"
+  using Derives1_prepend by (induction D arbitrary: b b') (auto, fast)
 
 lemma Derives1_append:
-  assumes "Derives1 u i r v"
-  shows "Derives1 (u@w) i r (v@w)"
+  assumes "Derives1 cfg u i r v"
+  shows "Derives1 cfg (u@w) i r (v@w)"
 proof -
   obtain x y N \<alpha> where *: 
     "u = x @ [N] @ y" "v = x @ \<alpha> @ y"
-    "(N, \<alpha>) \<in> set \<RR>" "r = (N, \<alpha>)" "i = length x"
-    using assms Derives1_def by blast
+    "(N, \<alpha>) \<in> set (\<RR> cfg)" "r = (N, \<alpha>)" "i = length x"
+    using assms Derives1_def by (smt (verit))
   hence "u@w = x @ [N] @ y @ w" "v@w = x @ \<alpha> @ y @ w"
     by auto
   thus ?thesis
@@ -124,42 +121,42 @@ proof -
 qed
 
 lemma Derivation_append':
-  "Derivation a D a' \<Longrightarrow> Derivation (a@b) D (a'@b)"
-  using Derives1_append by (induction D arbitrary: a a') (auto, blast)
+  "Derivation cfg a D a' \<Longrightarrow> Derivation cfg (a@b) D (a'@b)"
+  using Derives1_append by (induction D arbitrary: a a') (auto, fast)
 
 lemma Derivation_append_rewrite:
-  assumes "Derivation a D (b @ c @ d) " "Derivation c E c'"
-  shows "\<exists>F. Derivation a F (b @ c' @ d)"
+  assumes "Derivation cfg a D (b @ c @ d) " "Derivation cfg c E c'"
+  shows "\<exists>F. Derivation cfg a F (b @ c' @ d)"
   using assms Derivation_append' Derivation_prepend Derivation_implies_append by fast
 
 lemma derives1_if_valid_rule:
-  "(N, \<alpha>) \<in> set \<RR> \<Longrightarrow> derives1 [N] \<alpha>"
+  "(N, \<alpha>) \<in> set (\<RR> cfg) \<Longrightarrow> derives1 cfg [N] \<alpha>"
   unfolding derives1_def
   apply (rule_tac exI[where x="[]"])
   apply (rule_tac exI[where x="[]"])
   by simp
 
 lemma derives_if_valid_rule:
-  "(N, \<alpha>) \<in> set \<RR> \<Longrightarrow> derives [N] \<alpha>"
-  using derives1_if_valid_rule by simp
+  "(N, \<alpha>) \<in> set (\<RR> cfg) \<Longrightarrow> derives cfg [N] \<alpha>"
+  using derives1_if_valid_rule by fastforce
 
 lemma Derivation_from_empty:
-  "Derivation [] D a \<Longrightarrow> a = []"
+  "Derivation cfg [] D a \<Longrightarrow> a = []"
   by (cases D) (auto simp: Derives1_def)
 
 lemma Derivation_concat_split:
-  "Derivation (a@b) D c \<Longrightarrow> \<exists>E F a' b'. Derivation a E a' \<and> Derivation b F b' \<and>
+  "Derivation cfg (a@b) D c \<Longrightarrow> \<exists>E F a' b'. Derivation cfg a E a' \<and> Derivation cfg b F b' \<and>
      c = a' @ b' \<and> length E \<le> length D \<and> length F \<le> length D"
 proof (induction D arbitrary: a b)
   case Nil
   thus ?case
-    by (metis local.Derivation.simps(1) order_refl)
+    by (metis Derivation.simps(1) order_refl)
 next
   case (Cons d D)
-  then obtain ab where *: "Derives1 (a@b) (fst d) (snd d) ab" "Derivation ab D c"
+  then obtain ab where *: "Derives1 cfg (a@b) (fst d) (snd d) ab" "Derivation cfg ab D c"
     by auto
   then obtain x y N \<alpha> where #:
-    "a@b = x @ [N] @ y" "ab = x @ \<alpha> @ y" "(N,\<alpha>) \<in> set \<RR>" "snd d = (N,\<alpha>)" "fst d = length x"
+    "a@b = x @ [N] @ y" "ab = x @ \<alpha> @ y" "(N,\<alpha>) \<in> set (\<RR> cfg)" "snd d = (N,\<alpha>)" "fst d = length x"
     using * unfolding Derives1_def by blast
   show ?case
   proof (cases "length a \<le> length x")
@@ -170,17 +167,17 @@ next
       "ab = take (length a) x @ drop (length a) x @ \<alpha> @ y"
       using #(1,2) True by (metis append_eq_append_conv_if)+
     then obtain E F a' b' where IH:
-      "Derivation (take (length a) x) E a'"
-      "Derivation (drop (length a) x @ \<alpha> @ y) F b'"
+      "Derivation cfg (take (length a) x) E a'"
+      "Derivation cfg (drop (length a) x @ \<alpha> @ y) F b'"
       "c = a' @ b'"
       "length E \<le> length D"
       "length F \<le> length D"
       using Cons *(2) by blast
-    have "Derives1 b (fst d - length a) (snd d) (drop (length a) x @ \<alpha> @ y)"
+    have "Derives1 cfg b (fst d - length a) (snd d) (drop (length a) x @ \<alpha> @ y)"
       unfolding Derives1_def using *(1) #(3-5) ab_def(2) by (metis length_drop)
-    hence "Derivation b ((fst d - length a, snd d) # F) b'"
+    hence "Derivation cfg b ((fst d - length a, snd d) # F) b'"
       using IH(2) by force
-    moreover have "Derivation a E a'"
+    moreover have "Derivation cfg a E a'"
       using IH(1) ab_def(1) by fastforce
     ultimately show ?thesis
       using IH(3-5) by fastforce
@@ -194,25 +191,23 @@ next
     have "ab = x @ \<alpha> @ take (length a - length x - 1) y @ drop (length a - length x - 1) y"
       using #(2) by force
     then obtain E F a' b' where IH:
-      "Derivation (x @ \<alpha> @ take (length a - length x - 1) y) E a'"
-      "Derivation (drop (length a - length x - 1) y) F b'"
+      "Derivation cfg (x @ \<alpha> @ take (length a - length x - 1) y) E a'"
+      "Derivation cfg (drop (length a - length x - 1) y) F b'"
       "c = a' @ b'"
       "length E \<le> length D"
       "length F \<le> length D"
       using Cons.IH[of "x @ \<alpha> @ take (length a - length x - 1) y" "drop (length a - length x - 1) y"] *(2) by auto
-    have "Derives1 a (fst d) (snd d) (x @ \<alpha> @ take (length a - length x - 1) y)"
+    have "Derives1 cfg a (fst d) (snd d) (x @ \<alpha> @ take (length a - length x - 1) y)"
       unfolding Derives1_def using #(3-5) a_def by blast
-    hence "Derivation a ((fst d, snd d) # E) a'"
+    hence "Derivation cfg a ((fst d, snd d) # E) a'"
       using IH(1) by fastforce
-    moreover have "Derivation b F b'"
+    moreover have "Derivation cfg b F b'"
       using b_def IH(2) by blast
     ultimately show ?thesis
       using IH(3-5) by fastforce
   qed
 qed
 
-
-end
 
 section \<open>Earley recognizer\<close>
 
@@ -262,31 +257,28 @@ lemmas item_defs = item_rule_head_def item_rule_body_def item_\<alpha>_def item_
 definition bin :: "'a items \<Rightarrow> nat \<Rightarrow> 'a items" where
   "bin I k = { x . x \<in> I \<and> item_end x = k }"
 
-definition wf_item :: "'a rules \<Rightarrow> 'a list => 'a item \<Rightarrow> bool" where 
-  "wf_item \<RR> inp x = (
-    item_rule x \<in> set \<RR> \<and> 
+definition wf_item :: "'a cfg \<Rightarrow> 'a sentence => 'a item \<Rightarrow> bool" where 
+  "wf_item cfg inp x = (
+    item_rule x \<in> set (\<RR> cfg) \<and> 
     item_dot x \<le> length (item_rule_body x) \<and>
     item_origin x \<le> item_end x \<and> 
     item_end x \<le> length inp)"
 
-definition wf_items :: "'a rules \<Rightarrow> 'a list \<Rightarrow> 'a items \<Rightarrow> bool" where
-  "wf_items \<RR> inp I = (\<forall>x \<in> I. wf_item \<RR> inp x)"
+definition wf_items :: "'a cfg \<Rightarrow> 'a sentence \<Rightarrow> 'a items \<Rightarrow> bool" where
+  "wf_items cfg inp I = (\<forall>x \<in> I. wf_item cfg inp x)"
 
 subsection \<open>Epsilon Productions\<close>
 
-context CFG
-begin
-
-definition \<epsilon>_free :: "bool" where
-  "\<epsilon>_free = (\<forall>r \<in> set \<RR>. rule_body r \<noteq> [])"
+definition \<epsilon>_free :: "'a cfg \<Rightarrow> bool" where
+  "\<epsilon>_free cfg \<longleftrightarrow> (\<forall>r \<in> set (\<RR> cfg). rule_body r \<noteq> [])"
 
 lemma \<epsilon>_free_impl_non_empty_sentence_deriv:
-  "\<epsilon>_free \<Longrightarrow> a \<noteq> [] \<Longrightarrow> \<not> Derivation a D []"
+  "\<epsilon>_free cfg \<Longrightarrow> a \<noteq> [] \<Longrightarrow> \<not> Derivation cfg a D []"
 proof (induction "length D" arbitrary: a D rule: nat_less_induct)
   case 1
   show ?case
   proof (rule ccontr)
-    assume assm: "\<not> \<not> Derivation a D []"
+    assume assm: "\<not> \<not> Derivation cfg a D []"
     show False
     proof (cases "D = []")
       case True
@@ -295,8 +287,8 @@ proof (induction "length D" arbitrary: a D rule: nat_less_induct)
     next
       case False
       then obtain d D' \<alpha> where *:
-        "D = d # D'" "Derives1 a (fst d) (snd d) \<alpha>" "Derivation \<alpha> D' []" "snd d \<in> set \<RR>"
-        using list.exhaust assm Derives1_def by (metis local.Derivation.simps(2))
+        "D = d # D'" "Derives1 cfg a (fst d) (snd d) \<alpha>" "Derivation cfg \<alpha> D' []" "snd d \<in> set (\<RR> cfg)"
+        using list.exhaust assm Derives1_def by (metis Derivation.simps(2))
       show ?thesis
       proof cases
         assume "\<alpha> = []"
@@ -312,14 +304,14 @@ proof (induction "length D" arbitrary: a D rule: nat_less_induct)
 qed
 
 lemma \<epsilon>_free_impl_non_empty_deriv:
-  "\<epsilon>_free \<Longrightarrow> N \<in> set \<NN> \<Longrightarrow> \<not> derives [N] []"
-  using \<epsilon>_free_impl_non_empty_sentence_deriv derives_implies_Derivation is_nonterminal_def by (meson not_Cons_self2)
+  "\<epsilon>_free cfg \<Longrightarrow> N \<in> set (\<NN> cfg) \<Longrightarrow> \<not> derives cfg [N] []"
+  using \<epsilon>_free_impl_non_empty_sentence_deriv derives_implies_Derivation by (metis not_Cons_self2)
 
 
 subsection \<open>Earley algorithm\<close>
 
-definition Init :: "'a items" where
-  "Init = { init_item r 0 | r. r \<in> set \<RR> \<and> fst r = \<SS> }"
+definition Init :: "'a cfg \<Rightarrow> 'a items" where
+  "Init cfg = { init_item r 0 | r. r \<in> set (\<RR> cfg) \<and> fst r = (\<SS> cfg) }"
 
 definition Scan :: "nat \<Rightarrow> 'a sentence \<Rightarrow> 'a items \<Rightarrow> 'a items" where
   "Scan k inp I = 
@@ -329,10 +321,10 @@ definition Scan :: "nat \<Rightarrow> 'a sentence \<Rightarrow> 'a items \<Right
         k < length inp \<and>
         next_symbol x = Some a }"
 
-definition Predict :: "nat \<Rightarrow> 'a items \<Rightarrow> 'a items" where
-  "Predict k I =
+definition Predict :: "nat \<Rightarrow> 'a cfg \<Rightarrow> 'a items \<Rightarrow> 'a items" where
+  "Predict k cfg I =
     { init_item r k | r x.
-        r \<in> set \<RR> \<and>
+        r \<in> set (\<RR> cfg) \<and>
         x \<in> bin I k \<and>
         next_symbol x = Some (rule_head r) }"
 
@@ -344,114 +336,114 @@ definition Complete :: "nat \<Rightarrow> 'a items \<Rightarrow> 'a items" where
         is_complete y \<and>
         next_symbol x = Some (item_rule_head y) }"
 
-definition \<pi>_step :: "nat \<Rightarrow> 'a sentence \<Rightarrow> 'a items \<Rightarrow> 'a items" where
-  "\<pi>_step k inp I = I \<union> Scan k inp I \<union> Complete k I \<union> Predict k I"
+definition \<pi>_step :: "nat \<Rightarrow> 'a cfg \<Rightarrow> 'a sentence \<Rightarrow> 'a items \<Rightarrow> 'a items" where
+  "\<pi>_step k cfg inp I = I \<union> Scan k inp I \<union> Complete k I \<union> Predict k cfg I"
 
-definition \<pi> :: "nat \<Rightarrow> 'a sentence \<Rightarrow> 'a items \<Rightarrow> 'a items" where
-  "\<pi> k inp I = limit (\<pi>_step k inp) I"
+definition \<pi> :: "nat \<Rightarrow> 'a cfg \<Rightarrow> 'a sentence \<Rightarrow> 'a items \<Rightarrow> 'a items" where
+  "\<pi> k cfg inp I = limit (\<pi>_step k cfg inp) I"
 
-fun \<I> :: "nat \<Rightarrow> 'a sentence \<Rightarrow> 'a items" where
-  "\<I> 0 inp = \<pi> 0 inp Init"
-| "\<I> (Suc n) inp = \<pi> (Suc n) inp (\<I> n inp)"
+fun \<I> :: "nat \<Rightarrow> 'a cfg \<Rightarrow> 'a sentence \<Rightarrow> 'a items" where
+  "\<I> 0 cfg inp = \<pi> 0 cfg inp (Init cfg)"
+| "\<I> (Suc n) cfg inp = \<pi> (Suc n) cfg inp (\<I> n cfg inp)"
 
-definition \<II> :: "'a sentence \<Rightarrow> 'a items" where
-  "\<II> inp = \<I> (length inp) inp"
+definition \<II> :: "'a cfg \<Rightarrow> 'a sentence \<Rightarrow> 'a items" where
+  "\<II> cfg inp = \<I> (length inp) cfg inp"
 
-definition is_finished :: "'a sentence \<Rightarrow> 'a item \<Rightarrow> bool" where
-  "is_finished inp x \<longleftrightarrow> (
-    item_rule_head x = \<SS> \<and>
+definition is_finished :: "'a cfg \<Rightarrow> 'a sentence \<Rightarrow> 'a item \<Rightarrow> bool" where
+  "is_finished cfg inp x \<longleftrightarrow> (
+    item_rule_head x = \<SS> cfg \<and>
     item_origin x = 0 \<and>
     item_end x = length inp \<and> 
     is_complete x)"
 
-definition earley_recognized :: "'a sentence \<Rightarrow> bool" where
-  "earley_recognized inp = (\<exists>x \<in> \<II> inp. is_finished inp x)"
+definition earley_recognized :: "'a cfg \<Rightarrow> 'a sentence \<Rightarrow> bool" where
+  "earley_recognized cfg inp = (\<exists>x \<in> \<II> cfg inp. is_finished cfg inp x)"
 
 subsection \<open>Wellformedness\<close>
 
 lemma wf_items_Un:
-  "wf_items \<RR> inp I \<Longrightarrow> wf_items \<RR> inp J \<Longrightarrow> wf_items \<RR> inp (I \<union> J)"
+  "wf_items cfg inp I \<Longrightarrow> wf_items cfg inp J \<Longrightarrow> wf_items cfg inp (I \<union> J)"
   unfolding wf_items_def by blast
 
 lemmas wf_defs = wf_item_def wf_items_def
 
 lemma wf_Init:
-  "x \<in> Init \<Longrightarrow> wf_item \<RR> inp x"
+  "x \<in> Init cfg \<Longrightarrow> wf_item cfg inp x"
   unfolding Init_def wf_item_def init_item_def by auto
 
 lemma wf_Scan:
-  "wf_items \<RR> inp I \<Longrightarrow> wf_items \<RR> inp (Scan k inp I)"
+  "wf_items cfg inp I \<Longrightarrow> wf_items cfg inp (Scan k inp I)"
   unfolding Scan_def wf_defs bin_def inc_item_def is_complete_def item_rule_body_def next_symbol_def
   by (auto split: if_splits)
 
 lemma wf_Predict:
-  "wf_items \<RR> inp I \<Longrightarrow> wf_items \<RR> inp (Predict k I)"
+  "wf_items cfg inp I \<Longrightarrow> wf_items cfg inp (Predict k cfg I)"
   unfolding Predict_def wf_defs bin_def init_item_def by auto
 
 lemma wf_Complete:
-  "wf_items \<RR> inp I \<Longrightarrow> wf_items \<RR> inp (Complete k I)"
+  "wf_items cfg inp I \<Longrightarrow> wf_items cfg inp (Complete k I)"
   unfolding Complete_def wf_defs bin_def inc_item_def is_complete_def item_rule_body_def next_symbol_def
   by (auto split: if_splits; metis le_trans)
 
 lemma wf_\<pi>_step:
-  "wf_items \<RR> inp I \<Longrightarrow> wf_items \<RR> inp (\<pi>_step k inp I)"
-  unfolding \<pi>_step_def using wf_Scan wf_Predict wf_Complete wf_items_Un by simp
+  "wf_items cfg inp I \<Longrightarrow> wf_items cfg inp (\<pi>_step k cfg inp I)"
+  unfolding \<pi>_step_def using wf_Scan wf_Predict wf_Complete wf_items_Un by metis
 
 lemma wf_funpower:
-  "wf_items \<RR> inp I \<Longrightarrow> wf_items \<RR> inp (funpower (\<pi>_step k inp) n I)"
+  "wf_items cfg inp I \<Longrightarrow> wf_items cfg inp (funpower (\<pi>_step k cfg inp) n I)"
   using wf_\<pi>_step unfolding wf_items_def
-  by (induction n) auto
+  by (induction n) (auto, blast)
 
 lemma wf_\<pi>:
-  "wf_items \<RR> inp I \<Longrightarrow> wf_items \<RR> inp (\<pi> k inp I)"
+  "wf_items cfg inp I \<Longrightarrow> wf_items cfg inp (\<pi> k cfg inp I)"
   by (metis \<pi>_def elem_limit_simp wf_funpower wf_items_def)
 
 lemma wf_\<pi>0:
-  "wf_items \<RR> inp (\<pi> 0 inp Init)"
+  "wf_items cfg inp (\<pi> 0 cfg inp (Init cfg))"
   using wf_items_def wf_Init wf_\<pi> by metis
 
 lemma wf_\<I>:
-  "wf_items \<RR> inp (\<I> n inp)"
+  "wf_items cfg inp (\<I> n cfg inp)"
   by (induction n) (auto simp: wf_\<pi>0 wf_\<pi>)
 
 lemma wf_\<II>:
-  "wf_items \<RR> inp (\<II> inp)"
+  "wf_items cfg inp (\<II> cfg inp)"
   unfolding \<II>_def using wf_\<I> by blast
 
 subsection \<open>Soundness\<close>
 
-definition sound_item :: "'a sentence \<Rightarrow> 'a item \<Rightarrow> bool" where
-  "sound_item inp x = derives [item_rule_head x] (slice (item_origin x) (item_end x) inp @ item_\<beta> x)"
+definition sound_item :: "'a cfg \<Rightarrow> 'a sentence \<Rightarrow> 'a item \<Rightarrow> bool" where
+  "sound_item cfg inp x = derives cfg [item_rule_head x] (slice (item_origin x) (item_end x) inp @ item_\<beta> x)"
 
-definition sound_items :: "'a sentence \<Rightarrow> 'a items \<Rightarrow> bool" where
-  "sound_items inp I = (\<forall>x \<in> I. sound_item inp x)"
+definition sound_items :: "'a cfg \<Rightarrow> 'a sentence \<Rightarrow> 'a items \<Rightarrow> bool" where
+  "sound_items cfg inp I = (\<forall>x \<in> I. sound_item cfg inp x)"
 
 lemmas sound_defs = sound_items_def sound_item_def
 
 lemma sound_Init:
-  "sound_items inp Init"
+  "sound_items cfg inp (Init cfg)"
   unfolding sound_items_def
 proof (standard)
   fix x
-  assume *: "x \<in> Init"
+  assume *: "x \<in> Init cfg"
   hence "item_dot x = 0"
-    using Init_def by (auto, simp add: init_item_def)
-  hence "(item_rule_head x, item_\<beta> x) \<in> set \<RR>"
+    by (smt (verit) Init_def init_item_def item.exhaust_sel item.inject mem_Collect_eq)
+  hence "(item_rule_head x, item_\<beta> x) \<in> set (\<RR> cfg)"
     unfolding item_rule_head_def rule_head_def item_\<beta>_def item_rule_body_def rule_body_def
     using * wf_Init wf_item_def by fastforce
-  hence "derives [item_rule_head x] (item_\<beta> x)"
-    using derives_if_valid_rule by blast
+  hence "derives cfg [item_rule_head x] (item_\<beta> x)"
+    using derives_if_valid_rule by metis
   moreover have "item_origin x = item_end x"
-    using * Init_def by (auto, simp add: init_item_def)
-  ultimately show "sound_item inp x"
+    by (metis * Ex_list_of_length nle_le wf_Init wf_item_def)
+  ultimately show "sound_item cfg inp x"
     unfolding sound_item_def by (simp add: slice_empty)
 qed
 
 lemma sound_item_inc_item:
-  assumes "wf_item \<RR> inp x" "sound_item inp x"
+  assumes "wf_item cfg inp x" "sound_item cfg inp x"
   assumes "next_symbol x = Some a"
   assumes "k < length inp" "inp!k = a" "item_end x = k"
-  shows "sound_item inp (inc_item x (k+1))"
+  shows "sound_item cfg inp (inc_item x (k+1))"
 proof -
   define x' where [simp]: "x' = inc_item x (k+1)"
   obtain item_\<beta>' where *: "item_\<beta> x = a # item_\<beta>'"
@@ -461,28 +453,28 @@ proof -
     using * assms(1,4-6) slice_append_nth wf_item_def by (auto simp: inc_item_def; blast)
   moreover have "item_\<beta>' = item_\<beta> x'"
     using * by (auto simp: inc_item_def item_\<beta>_def item_rule_body_def, metis List.list.sel(3) drop_Suc tl_drop)
-  moreover have "derives [item_rule_head x] (slice (item_origin x) (item_end x) inp @ item_\<beta> x)"
+  moreover have "derives cfg [item_rule_head x] (slice (item_origin x) (item_end x) inp @ item_\<beta> x)"
     using assms(1,2,6) sound_item_def by blast
   ultimately show ?thesis
     by (simp add: inc_item_def item_rule_head_def sound_item_def)
 qed
 
 lemma sound_Scan:
-  "wf_items \<RR> inp I \<Longrightarrow> sound_items inp I \<Longrightarrow> sound_items inp (Scan k inp I)"
-  unfolding Scan_def using sound_item_inc_item by (auto simp: wf_items_def sound_items_def bin_def)
+  "wf_items cfg inp I \<Longrightarrow> sound_items cfg inp I \<Longrightarrow> sound_items cfg inp (Scan k inp I)"
+  unfolding Scan_def using sound_item_inc_item by (auto simp: wf_items_def sound_items_def bin_def; fast)
 
 lemma sound_Predict:
-  "sound_items inp I \<Longrightarrow> sound_items inp (Predict k I)"
+  "sound_items cfg inp I \<Longrightarrow> sound_items cfg inp (Predict k cfg I)"
   unfolding Predict_def by (auto simp: sound_defs init_item_def derives_if_valid_rule slice_empty item_defs)
 
 lemma sound_Complete:
-  assumes "wf_items \<RR> inp I" "sound_items inp I"
-  shows "sound_items inp (Complete k I)"
+  assumes "wf_items cfg inp I" "sound_items cfg inp I"
+  shows "sound_items cfg inp (Complete k I)"
   unfolding sound_items_def
 proof standard
   fix z
   assume "z \<in> Complete k I"
-  show "sound_item inp z"
+  show "sound_item cfg inp z"
   proof cases
     assume "z \<in> I"
     thus ?thesis
@@ -494,102 +486,102 @@ proof standard
       "is_complete y" "next_symbol x = Some (item_rule_head y)"
       using \<open>z \<in> Complete k I\<close> unfolding Complete_def by blast
 
-    have "derives [item_rule_head y] (slice (item_origin y) (item_end y) inp)"
-      using *(3,4) sound_defs assms by (auto simp: bin_def is_complete_def item_\<beta>_def)
-    then obtain E where E: "Derivation [item_rule_head y] E (slice (item_origin y) (item_end y) inp)"
+    have "derives cfg [item_rule_head y] (slice (item_origin y) (item_end y) inp)"
+      using *(3,4) sound_defs assms
+      by (metis (no_types, lifting) append_Nil2 bin_def drop_eq_Nil is_complete_def item_\<beta>_def mem_Collect_eq)
+    then obtain E where E: "Derivation cfg [item_rule_head y] E (slice (item_origin y) (item_end y) inp)"
       using derives_implies_Derivation by blast
 
-    have "derives [item_rule_head x] (slice (item_origin x) (item_origin y) inp @ item_\<beta> x)"
-      using *(2) sound_defs assms sound_items_def by (auto simp: bin_def)
+    have "derives cfg [item_rule_head x] (slice (item_origin x) (item_origin y) inp @ item_\<beta> x)"
+      using *(2) sound_defs assms sound_items_def by (metis (mono_tags, lifting) bin_def mem_Collect_eq)
     moreover have 0: "item_\<beta> x = (item_rule_head y) # tl (item_\<beta> x)"
       using *(5) by (auto simp: next_symbol_def item_\<beta>_def is_complete_def split: if_splits,
                      metis Cons_nth_drop_Suc drop_Suc drop_tl leI)
     ultimately obtain D where D: 
-      "Derivation [item_rule_head x] D (slice (item_origin x) (item_origin y) inp @
+      "Derivation cfg [item_rule_head x] D (slice (item_origin x) (item_origin y) inp @
        [item_rule_head y] @ (tl (item_\<beta> x)))"
       using derives_implies_Derivation by (metis append_Cons append_Nil)
 
-    have "wf_item \<RR> inp x"
+    have "wf_item cfg inp x"
       using *(2) assms(1) bin_def wf_items_def by (metis (mono_tags, lifting) mem_Collect_eq)
     obtain G where 
-      "Derivation [item_rule_head x] G (slice (item_origin x) (item_origin y) inp @
+      "Derivation cfg [item_rule_head x] G (slice (item_origin x) (item_origin y) inp @
        slice (item_origin y) (item_end y) inp @ tl (item_\<beta> x))"
       using Derivation_append_rewrite D E by blast
     moreover have "item_origin x \<le> item_origin y"
-      using *(2) \<open>wf_item \<RR> inp x\<close> wf_item_def by (auto simp: bin_def; force)
+      using *(2) \<open>wf_item cfg inp x\<close> wf_item_def by (auto simp: bin_def; force)
     moreover have "item_origin y \<le> item_end y"
       using *(3) wf_defs assms(1) by (auto simp: bin_def; blast)
-    ultimately have "derives [item_rule_head x] (slice (item_origin x) (item_end y) inp @ tl (item_\<beta> x))"
+    ultimately have "derives cfg [item_rule_head x] (slice (item_origin x) (item_end y) inp @ tl (item_\<beta> x))"
       by (metis Derivation_implies_derives append.assoc slice_concat)
     moreover have "tl (item_\<beta> x) = item_\<beta> z"
       using *(1,5) 0 by (auto simp: inc_item_def item_rule_body_def tl_drop drop_Suc item_\<beta>_def)
     ultimately show ?thesis
-      using sound_item_def *(1,3) by (auto simp: bin_def inc_item_def item_rule_head_def)
+      using sound_item_def *(1,3) by (metis (mono_tags, lifting) bin_def inc_item_def item.sel(1,3,4) item_defs(1) mem_Collect_eq)
   qed
 qed
 
 lemma sound_\<pi>_step:
-  "wf_items \<RR> inp I \<Longrightarrow> sound_items inp I \<Longrightarrow> sound_items inp (\<pi>_step k inp I)"
+  "wf_items cfg inp I \<Longrightarrow> sound_items cfg inp I \<Longrightarrow> sound_items cfg inp (\<pi>_step k cfg inp I)"
   unfolding \<pi>_step_def using sound_Scan sound_Predict sound_Complete by (metis UnE sound_items_def)
 
 lemma sound_funpower:
-  "wf_items \<RR> inp I \<Longrightarrow> sound_items inp I \<Longrightarrow> sound_items inp (funpower (\<pi>_step k inp) n I)"
+  "wf_items cfg inp I \<Longrightarrow> sound_items cfg inp I \<Longrightarrow> sound_items cfg inp (funpower (\<pi>_step k cfg inp) n I)"
   by (induction n) (auto simp: sound_\<pi>_step wf_\<pi>_step wf_funpower)
 
 lemma sound_\<pi>:
-  assumes "wf_items \<RR> inp I" "sound_items inp I"
-  shows "sound_items inp (\<pi> k inp I)"
+  assumes "wf_items cfg inp I" "sound_items cfg inp I"
+  shows "sound_items cfg inp (\<pi> k cfg inp I)"
   by (metis \<pi>_def assms elem_limit_simp sound_items_def sound_funpower)
 
 lemma sound_\<pi>0:
-  "sound_items inp (\<pi> 0 inp Init)"
-  using sound_items_def sound_Init sound_\<pi> wf_Init wf_items_def by metis
+  "sound_items cfg inp (\<pi> 0 cfg inp (Init cfg))"
+  using sound_Init sound_\<pi> wf_Init wf_items_def by metis
 
 lemma sound_\<I>:
-  "sound_items inp (\<I> k inp)"
+  "sound_items cfg inp (\<I> k cfg inp)"
   apply (induction k)
   apply (auto simp: sound_\<pi>0)
   using sound_\<pi> wf_\<I> by force
 
 lemma sound_\<II>:
-  "sound_items inp (\<II> inp)"
+  "sound_items cfg inp (\<II> cfg inp)"
   unfolding \<II>_def using sound_\<I> by blast
 
 theorem soundness:
-  "earley_recognized inp \<Longrightarrow> derives [\<SS>] inp"
+  "earley_recognized cfg inp \<Longrightarrow> derives cfg [\<SS> cfg] inp"
   using earley_recognized_def sound_\<II> sound_defs
-  apply (auto simp: is_complete_def is_finished_def item_\<beta>_def)
-  by (metis drop_all self_append_conv slice_id)
+  by (metis drop_eq_Nil is_complete_def is_finished_def item_\<beta>_def self_append_conv slice_id)
 
 subsection \<open>Monotonicity and Absorption\<close>
 
 lemma \<pi>_step_empty:
-  "\<pi>_step k inp {} = {}"
+  "\<pi>_step k cfg inp {} = {}"
   unfolding \<pi>_step_def Scan_def Complete_def Predict_def bin_def by blast
 
 lemma \<pi>_step_setmonotone:
-  "setmonotone (\<pi>_step k inp)"
+  "setmonotone (\<pi>_step k cfg inp)"
   by (simp add: Un_assoc \<pi>_step_def setmonotone_def)
 
 lemma \<pi>_step_continuous:
-  "continuous (\<pi>_step k inp)"
+  "continuous (\<pi>_step k cfg inp)"
   unfolding continuous_def
 proof (standard, standard, standard)
   fix C :: "nat \<Rightarrow> 'a item set"
   assume "chain C"
-  thus "chain (\<pi>_step k inp \<circ> C)"
+  thus "chain (\<pi>_step k cfg inp \<circ> C)"
     unfolding chain_def \<pi>_step_def by (auto simp: Scan_def Predict_def Complete_def bin_def subset_eq)
 next
   fix C :: "nat \<Rightarrow> 'a item set"
   assume *: "chain C"
-  show "\<pi>_step k inp (natUnion C) = natUnion (\<pi>_step k inp \<circ> C)"
+  show "\<pi>_step k cfg inp (natUnion C) = natUnion (\<pi>_step k cfg inp \<circ> C)"
     unfolding natUnion_def
   proof standard
-    show "\<pi>_step k inp (\<Union> {C n |n. True}) \<subseteq> \<Union> {(\<pi>_step k inp \<circ> C) n |n. True}"
+    show "\<pi>_step k cfg inp (\<Union> {C n |n. True}) \<subseteq> \<Union> {(\<pi>_step k cfg inp \<circ> C) n |n. True}"
     proof standard
       fix x
-      assume #: "x \<in> \<pi>_step k inp (\<Union> {C n |n. True})"
-      show "x \<in> \<Union> {(\<pi>_step k inp \<circ> C) n |n. True}"
+      assume #: "x \<in> \<pi>_step k cfg inp (\<Union> {C n |n. True})"
+      show "x \<in> \<Union> {(\<pi>_step k cfg inp \<circ> C) n |n. True}"
       proof (cases "x \<in> Complete k (\<Union> {C n |n. True})")
         case True
         then show ?thesis
@@ -620,7 +612,7 @@ next
                                 item_end j = item_end z \<and> 
                                 is_complete j \<and>
                                 next_symbol i = Some (item_rule_head j))} \<union>
-                           Predict (item_end z) (C n))
+                           Predict (item_end z) cfg (C n))
                   \<and> inc_item y (item_end z) \<in> I"
             using f7 a5 a2 a1 by blast
         qed
@@ -631,18 +623,18 @@ next
       qed
     qed
   next
-    show "\<Union> {(\<pi>_step k inp \<circ> C) n |n. True} \<subseteq> \<pi>_step k inp (\<Union> {C n |n. True})"
+    show "\<Union> {(\<pi>_step k cfg inp \<circ> C) n |n. True} \<subseteq> \<pi>_step k cfg inp (\<Union> {C n |n. True})"
       unfolding \<pi>_step_def
       using * by (auto simp: Scan_def Predict_def Complete_def chain_def bin_def, metis+)
   qed
 qed
 
 lemma \<pi>_step_regular:
-  "regular (\<pi>_step k inp)"
+  "regular (\<pi>_step k cfg inp)"
   by (simp add: \<pi>_step_continuous \<pi>_step_setmonotone regular_def)
 
 lemma \<pi>_idem:
-  "\<pi> k inp (\<pi> k inp I) = \<pi> k inp I"
+  "\<pi> k cfg inp (\<pi> k cfg inp I) = \<pi> k cfg inp I"
   by (simp add: \<pi>_def \<pi>_step_regular limit_is_idempotent)
 
 lemma Scan_bin_absorb:
@@ -650,7 +642,7 @@ lemma Scan_bin_absorb:
   unfolding Scan_def bin_def by simp
 
 lemma Predict_bin_absorb:
-  "Predict k (bin I k) = Predict k I"
+  "Predict k cfg (bin I k) = Predict k cfg I"
   unfolding Predict_def bin_def by simp
 
 lemma Complete_bin_absorb:
@@ -662,7 +654,7 @@ lemma Scan_Un:
   unfolding Scan_def bin_def by blast
 
 lemma Predict_Un:
-  "Predict k (I \<union> J) = Predict k I \<union> Predict k J"
+  "Predict k cfg (I \<union> J) = Predict k cfg I \<union> Predict k cfg J"
   unfolding Predict_def bin_def by blast
 
 lemma Scan_sub_mono:
@@ -670,7 +662,7 @@ lemma Scan_sub_mono:
   unfolding Scan_def bin_def by blast
 
 lemma Predict_sub_mono:
-  "I \<subseteq> J \<Longrightarrow> Predict k I \<subseteq> Predict k J"
+  "I \<subseteq> J \<Longrightarrow> Predict k cfg I \<subseteq> Predict k cfg J"
   unfolding Predict_def bin_def by blast
 
 lemma Complete_sub_mono:
@@ -678,69 +670,69 @@ lemma Complete_sub_mono:
   unfolding Complete_def bin_def by blast
 
 lemma \<pi>_step_sub_mono:
-  "I \<subseteq> J \<Longrightarrow> \<pi>_step k inp I \<subseteq> \<pi>_step k inp J"
-  unfolding \<pi>_step_def using Scan_sub_mono Predict_sub_mono Complete_sub_mono by (meson Un_mono)
+  "I \<subseteq> J \<Longrightarrow> \<pi>_step k cfg inp I \<subseteq> \<pi>_step k cfg inp J"
+  unfolding \<pi>_step_def using Scan_sub_mono Predict_sub_mono Complete_sub_mono by (metis sup.mono)
 
 lemma funpower_sub_mono:
-  "I \<subseteq> J \<Longrightarrow> funpower (\<pi>_step k inp) n I \<subseteq> funpower (\<pi>_step k inp) n J"
+  "I \<subseteq> J \<Longrightarrow> funpower (\<pi>_step k cfg inp) n I \<subseteq> funpower (\<pi>_step k cfg inp) n J"
   by (induction n) (auto simp: \<pi>_step_sub_mono)
 
 lemma \<pi>_sub_mono:
-  "I \<subseteq> J \<Longrightarrow> \<pi> k inp I \<subseteq> \<pi> k inp J"
+  "I \<subseteq> J \<Longrightarrow> \<pi> k cfg inp I \<subseteq> \<pi> k cfg inp J"
 proof standard
   fix x
-  assume "I \<subseteq> J" "x \<in> \<pi> k inp I"
-  then obtain n where "x \<in> funpower (\<pi>_step k inp) n I"
+  assume "I \<subseteq> J" "x \<in> \<pi> k cfg inp I"
+  then obtain n where "x \<in> funpower (\<pi>_step k cfg inp) n I"
     unfolding \<pi>_def limit_def natUnion_def by blast
-  hence "x \<in> funpower (\<pi>_step k inp) n J"
+  hence "x \<in> funpower (\<pi>_step k cfg inp) n J"
     using \<open>I \<subseteq> J\<close> funpower_sub_mono by blast
-  thus "x \<in> \<pi> k inp J"
+  thus "x \<in> \<pi> k cfg inp J"
     unfolding \<pi>_def limit_def natUnion_def by blast
 qed
 
 lemma Scan_\<pi>_step_mono:
-  "Scan k inp I \<subseteq> \<pi>_step k inp I"
-  using \<pi>_step_def by auto
+  "Scan k inp I \<subseteq> \<pi>_step k cfg inp I"
+  using \<pi>_step_def by blast
 
 lemma Predict_\<pi>_step_mono:
-  "Predict k I \<subseteq> \<pi>_step k inp I"
-  using \<pi>_step_def by auto
+  "Predict k cfg I \<subseteq> \<pi>_step k cfg inp I"
+  using \<pi>_step_def by blast
 
 lemma Complete_\<pi>_step_mono:
-  "Complete k I \<subseteq> \<pi>_step k inp I"
-  using \<pi>_step_def by auto
+  "Complete k I \<subseteq> \<pi>_step k cfg inp I"
+  using \<pi>_step_def by blast
 
 lemma \<pi>_step_\<pi>_mono:
-  "\<pi>_step k inp I \<subseteq> \<pi> k inp I"
+  "\<pi>_step k cfg inp I \<subseteq> \<pi> k cfg inp I"
 proof -
-  have "\<pi>_step k inp I \<subseteq> funpower (\<pi>_step k inp) 1 I"
+  have "\<pi>_step k cfg inp I \<subseteq> funpower (\<pi>_step k cfg inp) 1 I"
     by simp
   thus ?thesis
     by (metis \<pi>_def limit_elem subset_eq)
 qed
 
 lemma Scan_\<pi>_mono:
-  "Scan k inp  I \<subseteq> \<pi> k inp I"
+  "Scan k inp  I \<subseteq> \<pi> k cfg inp I"
   using Scan_\<pi>_step_mono \<pi>_step_\<pi>_mono by force
 
 lemma Predict_\<pi>_mono:
-  "Predict k I \<subseteq> \<pi> k inp I"
+  "Predict k cfg I \<subseteq> \<pi> k cfg inp I"
   using Predict_\<pi>_step_mono \<pi>_step_\<pi>_mono by force
 
 lemma Complete_\<pi>_mono:
-  "Complete k I \<subseteq> \<pi> k inp I"
+  "Complete k I \<subseteq> \<pi> k cfg inp I"
   using Complete_\<pi>_step_mono \<pi>_step_\<pi>_mono by force
 
 lemma \<pi>_mono:
-  "I \<subseteq> \<pi> k inp I"
-  using \<pi>_step_\<pi>_mono \<pi>_step_def by auto
+  "I \<subseteq> \<pi> k cfg inp I"
+  using \<pi>_step_\<pi>_mono \<pi>_step_def by blast
 
 lemma Scan_bin_empty:
   "i \<noteq> k \<Longrightarrow> i \<noteq> k+1 \<Longrightarrow> bin (Scan k inp I) i = {}"
   unfolding Scan_def bin_def inc_item_def by fastforce
 
 lemma Predict_bin_empty:
-  "i \<noteq> k \<Longrightarrow> bin (Predict k I) i = {}"
+  "i \<noteq> k \<Longrightarrow> bin (Predict k cfg I) i = {}"
   unfolding Predict_def bin_def init_item_def by auto
 
 lemma Complete_bin_empty:
@@ -748,70 +740,70 @@ lemma Complete_bin_empty:
   unfolding Complete_def bin_def inc_item_def by auto
 
 lemma \<pi>_step_bin_absorb:
-  "i \<noteq> k \<Longrightarrow> i \<noteq> k + 1 \<Longrightarrow> bin (\<pi>_step k inp I) i = bin I i"
+  "i \<noteq> k \<Longrightarrow> i \<noteq> k + 1 \<Longrightarrow> bin (\<pi>_step k cfg inp I) i = bin I i"
   unfolding \<pi>_step_def using Scan_bin_empty Predict_bin_empty Complete_bin_empty
   unfolding bin_def using Un_iff empty_iff mem_Collect_eq by fastforce
 
 lemma funpower_bin_absorb:
-  "i \<noteq> k \<Longrightarrow> i \<noteq> k+1 \<Longrightarrow> bin (funpower (\<pi>_step k inp) n I) i = bin I i"
+  "i \<noteq> k \<Longrightarrow> i \<noteq> k+1 \<Longrightarrow> bin (funpower (\<pi>_step k cfg inp) n I) i = bin I i"
   by (induction n) (auto simp: \<pi>_step_bin_absorb)
 
 lemma \<pi>_bin_absorb:
   assumes "i \<noteq> k" "i \<noteq> k+1" 
-  shows "bin (\<pi> k inp I) i = bin I i"
+  shows "bin (\<pi> k cfg inp I) i = bin I i"
 proof (standard; standard)
   fix x 
-  assume "x \<in> bin (\<pi> k inp I) i"
-  then obtain n where "x \<in> bin (funpower (\<pi>_step k inp) n I) i"
+  assume "x \<in> bin (\<pi> k cfg inp I) i"
+  then obtain n where "x \<in> bin (funpower (\<pi>_step k cfg inp) n I) i"
     unfolding \<pi>_def limit_def natUnion_def by (auto simp: bin_def)
   then show "x \<in> bin I i"
     using funpower_bin_absorb assms by blast
 next
   fix x
   assume "x \<in> bin I i"
-  show "x \<in> bin (\<pi> k inp I) i"
-    using \<pi>_mono \<open>x \<in> bin I i\<close> by (auto simp: bin_def)
+  show "x \<in> bin (\<pi> k cfg inp I) i"
+    using \<pi>_mono \<open>x \<in> bin I i\<close> by (metis (no_types, lifting) bin_def mem_Collect_eq subsetD)
 qed
 
 subsection \<open>Completeness\<close>
 
 lemma Scan_\<I>:
-  assumes "i+1 \<le> k" "k \<le> length inp" "x \<in> bin (\<I> k inp) i" "next_symbol x = Some a" "inp!i = a"
-  shows "inc_item x (i+1) \<in> \<I> k inp"
+  assumes "i+1 \<le> k" "k \<le> length inp" "x \<in> bin (\<I> k cfg inp) i" "next_symbol x = Some a" "inp!i = a"
+  shows "inc_item x (i+1) \<in> \<I> k cfg inp"
   using assms
 proof (induction k arbitrary: i x a)
   case (Suc k)
   show ?case
   proof cases
     assume "i+1 \<le> k"
-    hence "inc_item x (i+1) \<in> \<I> k inp"
-      using Suc \<pi>_bin_absorb by simp
+    hence "inc_item x (i+1) \<in> \<I> k cfg inp"
+      using Suc \<pi>_bin_absorb by (metis \<I>.simps(2) add_leE leD le_imp_less_Suc plus_1_eq_Suc)
     thus ?thesis
       using \<pi>_mono unfolding Scan_def by force
   next
     assume "\<not> i+1 \<le> k"
     hence *: "i+1 = Suc k"
       using le_Suc_eq Suc.prems(1) by blast
-    have "x \<in> bin (\<I> k inp) i"
-      using Suc.prems(3) * \<pi>_bin_absorb by force
-    hence "inc_item x (i+1) \<in> \<pi> i inp (\<I> k inp)"
+    have "x \<in> bin (\<I> k cfg inp) i"
+      using Suc.prems(3) * \<pi>_bin_absorb by (metis Suc_eq_plus1 \<I>.simps(2) less_add_Suc2 nless_le plus_1_eq_Suc)
+    hence "inc_item x (i+1) \<in> \<pi> i cfg inp (\<I> k cfg inp)"
       using * Suc.prems(2,4,5) Scan_\<pi>_mono unfolding Scan_def by force
-    hence "inc_item x (i+1) \<in> \<pi> k inp (\<I> k inp)"
+    hence "inc_item x (i+1) \<in> \<pi> k cfg inp (\<I> k cfg inp)"
       using * by force
-    hence "inc_item x (i+1) \<in> \<I> k inp"
-      using \<pi>_idem by (metis local.\<I>.elims)
+    hence "inc_item x (i+1) \<in> \<I> k cfg inp"
+      using \<pi>_idem by (metis \<I>.elims)
     thus ?thesis
-      using \<pi>_mono by auto
+      using \<pi>_mono by force
   qed
 qed simp
 
 lemma Predict_\<I>:
-  assumes "i \<le> k" "x \<in> bin (\<I> k inp) i" "next_symbol x = Some N" "(N,\<alpha>) \<in> set \<RR>"
-  shows "init_item (N,\<alpha>) i \<in> \<I> k inp"
+  assumes "i \<le> k" "x \<in> bin (\<I> k cfg inp) i" "next_symbol x = Some N" "(N,\<alpha>) \<in> set (\<RR> cfg)"
+  shows "init_item (N,\<alpha>) i \<in> \<I> k cfg inp"
   using assms
 proof (induction k arbitrary: i x N \<alpha>)
   case 0
-  hence "init_item (N,\<alpha>) i \<in> Predict 0 (\<I> 0 inp)"
+  hence "init_item (N,\<alpha>) i \<in> Predict 0 cfg (\<I> 0 cfg inp)"
     unfolding rule_head_def Predict_def by auto
   thus ?case
     using Predict_\<pi>_mono \<pi>_idem by fastforce
@@ -820,13 +812,13 @@ next
   show ?case
   proof cases
     assume "i \<le> k"
-    hence "init_item (N,\<alpha>) i \<in> \<I> k inp"
-      using Suc.IH \<pi>_bin_absorb Suc.prems(2-4) by force
+    hence "init_item (N,\<alpha>) i \<in> \<I> k cfg inp"
+      using Suc.IH \<pi>_bin_absorb Suc.prems(2-4) by (metis \<I>.simps(2) add.commute le_imp_less_Suc nless_le plus_1_eq_Suc)
     thus ?thesis
-      using \<pi>_mono by auto
+      using \<pi>_mono by fastforce
   next
     assume "\<not> i \<le> k"
-    hence "init_item (N,\<alpha>) i \<in> Predict i (\<I> (Suc k) inp)"
+    hence "init_item (N,\<alpha>) i \<in> Predict i cfg (\<I> (Suc k) cfg inp)"
       unfolding Predict_def rule_head_def using Suc.prems(2-4) by auto
     thus ?thesis
       using Predict_\<pi>_mono \<pi>_idem Suc.prems(1) \<open>\<not> i \<le> k\<close> by (metis le_SucE \<I>.simps(2) subsetD)
@@ -834,13 +826,13 @@ next
 qed
 
 lemma Complete_\<I>:
-  assumes "i \<le> j" "j \<le> k" "x \<in> bin (\<I> k inp) i" "next_symbol x = Some N" "(N,\<alpha>) \<in> set \<RR>"
-  assumes "i = item_origin y" "y \<in> bin (\<I> k inp) j" "item_rule y = (N,\<alpha>)" "is_complete y"
-  shows "inc_item x j \<in> \<I> k inp"
+  assumes "i \<le> j" "j \<le> k" "x \<in> bin (\<I> k cfg inp) i" "next_symbol x = Some N" "(N,\<alpha>) \<in> set (\<RR> cfg)"
+  assumes "i = item_origin y" "y \<in> bin (\<I> k cfg inp) j" "item_rule y = (N,\<alpha>)" "is_complete y"
+  shows "inc_item x j \<in> \<I> k cfg inp"
   using assms
 proof (induction k arbitrary: i j x N \<alpha> y)
   case 0
-  hence "inc_item x 0 \<in> Complete 0 (\<I> 0 inp)"
+  hence "inc_item x 0 \<in> Complete 0 (\<I> 0 cfg inp)"
     unfolding Complete_def rule_head_def next_symbol_def item_rule_head_def by (auto split: if_splits; force)
   thus ?case
     using Complete_\<pi>_mono \<pi>_idem "0.prems"(2) by (metis le_0_eq \<I>.simps(1) subset_iff)
@@ -849,35 +841,35 @@ next
   show ?case
   proof cases
     assume "j \<le> k"
-    hence "inc_item x j \<in> \<I> k inp"
-      using Suc  \<pi>_bin_absorb Orderings.order_class.dual_order.eq_iff by force
+    hence "inc_item x j \<in> \<I> k cfg inp"
+      using Suc  \<pi>_bin_absorb Orderings.order_class.dual_order.eq_iff by (metis Suc_eq_plus1 \<I>.simps(2) not_less_eq_eq)
     thus ?thesis
       using \<pi>_mono by fastforce
   next
     assume "\<not> j \<le> k"
     hence "j = Suc k"
       using le_SucE Suc.prems(2) by blast
-    hence "inc_item x (Suc k) \<in> Complete (Suc k) (\<I> (Suc k) inp)"
+    hence "inc_item x (Suc k) \<in> Complete (Suc k) (\<I> (Suc k) cfg inp)"
       using Suc.prems(3-4,6-9) unfolding Complete_def rule_head_def item_rule_head_def by fastforce
     then show ?thesis
       using Complete_\<pi>_mono \<pi>_idem \<open>j = Suc k\<close> by fastforce
   qed
 qed
 
-definition partially_complete :: "nat \<Rightarrow> 'a sentence \<Rightarrow> 'a items \<Rightarrow> ('a derivation \<Rightarrow> bool) \<Rightarrow> bool" where
-  "partially_complete k inp I P = (
+definition partially_complete :: "nat \<Rightarrow> 'a cfg \<Rightarrow> 'a sentence \<Rightarrow> 'a items \<Rightarrow> ('a derivation \<Rightarrow> bool) \<Rightarrow> bool" where
+  "partially_complete k cfg inp I P = (
     \<forall>i j x a D.
       i \<le> j \<and> j \<le> k \<and> k \<le> length inp \<and>
       x \<in> bin I i \<and> next_symbol x = Some a \<and>
-      Derivation [a] D (slice i j inp) \<and> P D \<longrightarrow>
+      Derivation cfg [a] D (slice i j inp) \<and> P D \<longrightarrow>
       inc_item x j \<in> I
   )"
 
 lemma fully_complete:
   assumes "j \<le> k" "k \<le> length inp"
-  assumes "x = Item (N,\<alpha>) d i j" "x \<in> I" "wf_items \<RR> inp I"
-  assumes "Derivation (item_\<beta> x) D (slice j k inp)"
-  assumes "partially_complete k inp I (\<lambda>D'. length D' \<le> length D)"
+  assumes "x = Item (N,\<alpha>) d i j" "x \<in> I" "wf_items cfg inp I"
+  assumes "Derivation cfg (item_\<beta> x) D (slice j k inp)"
+  assumes "partially_complete k cfg inp I (\<lambda>D'. length D' \<le> length D)"
   shows "Item (N,\<alpha>) (length \<alpha>) i k \<in> I"
   using assms
 proof (induction "item_\<beta> x" arbitrary: d i j k N \<alpha> x D)
@@ -887,7 +879,7 @@ proof (induction "item_\<beta> x" arbitrary: d i j k N \<alpha> x D)
   hence "x = Item (N,\<alpha>) (length \<alpha>) i j"
     using Nil.hyps Nil.prems(3,4,5)
     unfolding wf_items_def wf_item_def rule_body_def item_rule_body_def item_defs(4) by auto
-  have "Derivation [] D (slice j k inp)"
+  have "Derivation cfg [] D (slice j k inp)"
     using Nil.hyps Nil.prems(6) by simp
   hence "slice j k inp = []"
     using Derivation_from_empty by blast
@@ -898,10 +890,10 @@ proof (induction "item_\<beta> x" arbitrary: d i j k N \<alpha> x D)
 next
   case (Cons b bs)
   then obtain j' E F where *: 
-    "Derivation [b] E (slice j j' inp)"
-    "Derivation bs F (slice j' k inp)"
+    "Derivation cfg [b] E (slice j j' inp)"
+    "Derivation cfg bs F (slice j' k inp)"
     "j \<le> j'" "j' \<le> k" "length E \<le> length D" "length F \<le> length D"
-    using Derivation_concat_split[of "[b]" bs D "slice j k inp"] slice_concat_Ex
+    using Derivation_concat_split[of cfg "[b]" bs D "slice j k inp"] slice_concat_Ex
     by (metis append_Cons append_Nil Cons.prems(1))
   have "x \<in> bin I j"
     using Cons.prems(3,4) by (auto simp: bin_def)
@@ -909,7 +901,7 @@ next
     using Cons unfolding item_defs(4) next_symbol_def is_complete_def by (auto, metis nth_via_drop)
   ultimately have "inc_item x j' \<in> I"
     using *(1,3-5) Cons.prems(2-4,7) partially_complete_def by metis
-  moreover have "partially_complete k inp I (\<lambda>D'. length D' \<le> length F)"
+  moreover have "partially_complete k cfg inp I (\<lambda>D'. length D' \<le> length F)"
     using Cons.prems(7) *(6) unfolding partially_complete_def by fastforce
   moreover have "bs = item_\<beta> (Item (N,\<alpha>) (d+1) i j')"
     using Cons.hyps(2) Cons.prems(3) unfolding item_defs(4) item_rule_body_def 
@@ -919,15 +911,16 @@ next
 qed
 
 lemma partially_complete_\<I>:
-  "partially_complete k inp (\<I> k inp) (\<lambda>_. True)"
+  assumes "wf_cfg cfg"
+  shows "partially_complete k cfg inp (\<I> k cfg inp) (\<lambda>_. True)"
   unfolding partially_complete_def
 proof (standard, standard, standard, standard, standard, standard)
   fix x i a D j
   assume
     "i \<le> j \<and> j \<le> k \<and> k \<le> length inp \<and>
-     x \<in> bin (\<I> k inp) i \<and> next_symbol x = Some a \<and>
-     Derivation [a] D (slice i j inp) \<and> (\<lambda>_. True) D"
-  thus "inc_item x j \<in> \<I> k inp"
+     x \<in> bin (\<I> k cfg inp) i \<and> next_symbol x = Some a \<and>
+     Derivation cfg [a] D (slice i j inp) \<and> (\<lambda>_. True) D"
+  thus "inc_item x j \<in> \<I> k cfg inp"
   proof (induction "length D" arbitrary: x i a j D rule: nat_less_induct)
     case 1
     show ?case
@@ -943,48 +936,48 @@ proof (standard, standard, standard, standard, standard, standard)
         using \<open>j \<le> length inp\<close> discrete by blast
       hence "inp!i = a"
         using slice_nth \<open>[a] = slice i j inp\<close> \<open>j = i + 1\<close> by fastforce
-      hence "inc_item x (i+1) \<in> \<I> k inp"
-        using Scan_\<I> \<open>j = i + 1\<close> "1.prems" by blast
+      hence "inc_item x (i+1) \<in> \<I> k cfg inp"
+        using Scan_\<I> \<open>j = i + 1\<close> "1.prems" by fast
       thus ?thesis
         by (simp add: \<open>j = i + 1\<close> wf_Init wf_items_def)
     next
       assume "\<not> D = []"
       then obtain d D' where "D = d # D'"
         by (meson List.list.exhaust)
-      then obtain b where *: "Derives1 [a] (fst d) (snd d) b" "Derivation b D' (slice i j inp)"
+      then obtain b where *: "Derives1 cfg [a] (fst d) (snd d) b" "Derivation cfg b D' (slice i j inp)"
         using "1.prems" by auto
       show ?thesis
       proof cases
-        assume "is_terminal a"
-        then obtain N \<alpha> where "[a] = [N]" "(N,\<alpha>) \<in> set \<RR>"
+        assume "is_terminal cfg a"
+        then obtain N \<alpha> where "[a] = [N]" "(N,\<alpha>) \<in> set (\<RR> cfg)"
           using *(1) unfolding Derives1_def by (metis Cons_eq_append_conv neq_Nil_conv)
-         hence "is_nonterminal a"
-           by simp
+         hence "is_nonterminal cfg a"
+           by (simp add: assms)
          thus ?thesis
-          using \<open>is_terminal a\<close> is_terminal_nonterminal by blast
+          using \<open>is_terminal cfg a\<close> is_terminal_nonterminal by (metis assms)
       next
-        assume "\<not> is_terminal a"
-        then obtain N \<alpha> where #: "[a] = [N]" "b = \<alpha>" "(N,\<alpha>) \<in> set \<RR>" "fst d = 0" "snd d = (N,\<alpha>)"
+        assume "\<not> is_terminal cfg a"
+        then obtain N \<alpha> where #: "[a] = [N]" "b = \<alpha>" "(N,\<alpha>) \<in> set (\<RR> cfg)" "fst d = 0" "snd d = (N,\<alpha>)"
           using *(1) unfolding Derives1_def by (simp add: Cons_eq_append_conv)
         define y where y_def: "y = Item (N,\<alpha>) 0 i i"
-        have "init_item (N, \<alpha>) i \<in> \<I> k inp"
-          using Predict_\<I> #(1,3) "1.prems" by auto
-        hence "y \<in> bin (\<I> k inp) i"
+        have "init_item (N, \<alpha>) i \<in> \<I> k cfg inp"
+          using Predict_\<I> #(1,3) "1.prems" by (metis (no_types, lifting) le_trans list.inject)
+        hence "y \<in> bin (\<I> k cfg inp) i"
           unfolding init_item_def using y_def by (simp add: bin_def wf_Init wf_items_def)
         have "length D' < length D"
           using \<open>D = d # D'\<close> by fastforce
-        hence "partially_complete k inp (\<I> k inp) (\<lambda>E. length E \<le> length D')"
+        hence "partially_complete k cfg inp (\<I> k cfg inp) (\<lambda>E. length E \<le> length D')"
           unfolding partially_complete_def using "1.hyps" "1.prems" le_less_trans by blast
-        hence "partially_complete j inp (\<I> k inp) (\<lambda>E. length E \<le> length D')"
+        hence "partially_complete j cfg inp (\<I> k cfg inp) (\<lambda>E. length E \<le> length D')"
           unfolding partially_complete_def using "1.prems" by force
-        moreover have "Derivation (item_\<beta> y) D' (slice i j inp)"
+        moreover have "Derivation cfg (item_\<beta> y) D' (slice i j inp)"
           using #(2) *(2) item_\<beta>_def item_rule_body_def rule_body_def y_def
           by (metis item.sel(1) item.sel(2) drop0 snd_conv)
-        ultimately have 0: "Item (N,\<alpha>) (length \<alpha>) i j \<in> bin (\<I> k inp) j"
-          using fully_complete wf_\<I> "1.prems" wf_items_def \<open>y \<in> bin (\<I> k inp) i\<close>
+        ultimately have 0: "Item (N,\<alpha>) (length \<alpha>) i j \<in> bin (\<I> k cfg inp) j"
+          using fully_complete wf_\<I> "1.prems" wf_items_def \<open>y \<in> bin (\<I> k cfg inp) i\<close>
           apply (auto simp: bin_def y_def)
-          by (smt (verit, best) fully_complete le_trans partially_complete_def)
-        have 1: "x \<in> bin (\<I> k inp) i"
+          using fully_complete le_trans partially_complete_def by (smt (verit, best) wf_\<I>)
+        have 1: "x \<in> bin (\<I> k cfg inp) i"
           by (simp add: "1.prems")
         have "next_symbol x = Some N"
           using #(1) "1.prems" by fastforce
@@ -996,46 +989,47 @@ proof (standard, standard, standard, standard, standard, standard)
 qed
 
 lemma partially_complete_\<II>:
-  "partially_complete (length inp) inp (\<II> inp) (\<lambda>_. True)"
+  "wf_cfg cfg \<Longrightarrow> partially_complete (length inp) cfg inp (\<II> cfg inp) (\<lambda>_. True)"
   by (simp add: \<II>_def partially_complete_\<I>)
 
 lemma Init_sub_\<I>:
-  "Init \<subseteq> \<I> k inp"
-  using \<pi>_mono by (induction k) (auto, blast)
+  "Init cfg \<subseteq> \<I> k cfg inp"
+  using \<pi>_mono by (induction k) (auto, blast, blast)
 
 lemma Derivation_\<SS>1:
-  assumes "Derivation [\<SS>] D inp" "set inp \<subseteq> set \<TT>"
-  shows "\<exists>\<alpha> E. Derivation \<alpha> E inp \<and> (\<SS>,\<alpha>) \<in> set \<RR>"
+  assumes "Derivation cfg [\<SS> cfg] D inp" "set inp \<subseteq> set (\<TT> cfg)" "wf_cfg cfg"
+  shows "\<exists>\<alpha> E. Derivation cfg \<alpha> E inp \<and> (\<SS> cfg,\<alpha>) \<in> set (\<RR> cfg)"
 proof (cases D)
   case Nil
   thus ?thesis
-    using assms is_nonterminal_startsymbol is_terminal_def is_terminal_nonterminal by fastforce
+    using assms is_nonterminal_startsymbol is_terminal_def is_terminal_nonterminal wf_cfg_defs by fastforce
 next
   case (Cons d D)
-  then obtain \<alpha> where "Derives1 [\<SS>] (fst d) (snd d) \<alpha>" "Derivation \<alpha> D inp"
+  then obtain \<alpha> where "Derives1 cfg [\<SS> cfg] (fst d) (snd d) \<alpha>" "Derivation cfg \<alpha> D inp"
     using assms by auto
-  hence "(\<SS>, \<alpha>) \<in> set \<RR>"
+  hence "(\<SS> cfg, \<alpha>) \<in> set (\<RR> cfg)"
     unfolding Derives1_def
     by (metis List.append.right_neutral List.list.discI append_eq_Cons_conv append_is_Nil_conv nth_Cons_0 self_append_conv2)
   thus ?thesis
-    using \<open>Derivation \<alpha> D inp\<close> by auto
+    using \<open>Derivation cfg \<alpha> D inp\<close> by auto
 qed
 
 theorem completeness:
-  assumes "derives [\<SS>] inp" "set inp \<subseteq> set \<TT>"
-  shows "earley_recognized inp"
+  assumes "derives cfg [\<SS> cfg] inp" "set inp \<subseteq> set (\<TT> cfg)" "wf_cfg cfg"
+  shows "earley_recognized cfg inp"
 proof -
-  obtain \<alpha> where *: "(\<SS>,\<alpha>) \<in> set \<RR>" "derives \<alpha> inp"
-    using Derivation_\<SS>1 assms Derivation_implies_derives derives_implies_Derivation by blast
-  let ?x = "Item (\<SS>,\<alpha>) 0 0 0"
-  have "?x \<in> \<II> inp" "wf_item \<RR> inp ?x"
-    unfolding \<II>_def using *(1) Init_sub_\<I> Init_def wf_Init by (auto simp: init_item_def)
-  moreover have "derives (item_\<beta> ?x) (slice 0 (length inp) inp)"
+  obtain \<alpha> where *: "(\<SS> cfg,\<alpha>) \<in> set (\<RR> cfg)" "derives cfg \<alpha> inp"
+    using Derivation_\<SS>1 assms Derivation_implies_derives derives_implies_Derivation by metis
+  let ?x = "Item (\<SS> cfg,\<alpha>) 0 0 0"
+  have "?x \<in> \<II> cfg inp" "wf_item cfg inp ?x"
+    unfolding \<II>_def using *(1) Init_sub_\<I> Init_def wf_Init by (auto simp: init_item_def, fast, fast)
+  moreover have "derives cfg (item_\<beta> ?x) (slice 0 (length inp) inp)"
     using *(2) item_defs(4) by (simp add: item_\<beta>_def item_rule_body_def rule_body_def)
-  ultimately have "Item (\<SS>,\<alpha>) (length \<alpha>) 0 (length inp) \<in> \<II> inp"
+  ultimately have "Item (\<SS> cfg,\<alpha>) (length \<alpha>) 0 (length inp) \<in> \<II> cfg inp"
     using partially_complete_\<II> fully_complete unfolding partially_complete_def 
     using fully_complete wf_\<II> derives_implies_Derivation
-    by (auto, metis Earley_Set.item.sel(4) le_refl slice_id wf_defs(1))
+    apply (auto)
+    by (smt (verit, ccfv_SIG) assms derives_implies_Derivation fully_complete length_0_conv nat_le_linear partially_complete_\<II> partially_complete_def slice_empty slice_id wf_\<II>)
   then show ?thesis
     unfolding earley_recognized_def is_finished_def by (auto simp: is_complete_def item_defs, force)
 qed
@@ -1043,42 +1037,42 @@ qed
 subsection \<open>Correctness\<close>
 
 corollary correctness:
-  assumes "set inp \<subseteq> set \<TT>"
-  shows "earley_recognized inp \<longleftrightarrow> derives [\<SS>] inp"
+  assumes "set inp \<subseteq> set (\<TT> cfg)" "wf_cfg cfg"
+  shows "earley_recognized cfg inp \<longleftrightarrow> derives cfg [\<SS> cfg] inp"
   using assms soundness completeness by blast
 
 subsection \<open>Finiteness\<close>
 
 lemma finiteness_empty:
-  "set \<RR> = {} \<Longrightarrow> finite { x | x. wf_item \<RR> inp x }"
+  "set (\<RR> cfg) = {} \<Longrightarrow> finite { x | x. wf_item cfg inp x }"
   unfolding wf_item_def by simp
 
 fun f :: "'a rule \<times> nat \<times> nat \<times> nat \<Rightarrow> 'a item" where
   "f (rule, dot, origin, ends) = Item rule dot origin ends" 
 
 lemma finiteness_nonempty:
-  assumes "set \<RR> \<noteq> {}"
-  shows "finite { x | x. wf_item \<RR> inp x }"
+  assumes "set (\<RR> cfg) \<noteq> {}"
+  shows "finite { x | x. wf_item cfg inp x }"
 proof -
-  define M where "M = Max { length (rule_body r) | r. r \<in> set \<RR> }"
-  define Top where "Top = (set \<RR> \<times> {0..M} \<times> {0..length inp} \<times> {0..length inp})"
+  define M where "M = Max { length (rule_body r) | r. r \<in> set (\<RR> cfg) }"
+  define Top where "Top = (set (\<RR> cfg) \<times> {0..M} \<times> {0..length inp} \<times> {0..length inp})"
   hence "finite Top"
     using finite_cartesian_product finite by blast
   have "inj_on f Top"
     unfolding Top_def inj_on_def by simp
   hence "finite (f ` Top)"
     using finite_image_iff \<open>finite Top\<close> by auto
-  have "{ x | x. wf_item \<RR> inp x } \<subseteq> f ` Top"
+  have "{ x | x. wf_item cfg inp x } \<subseteq> f ` Top"
   proof standard
     fix x
-    assume "x \<in> { x | x. wf_item \<RR> inp x }"
+    assume "x \<in> { x | x. wf_item cfg inp x }"
     then obtain rule dot origin endp where *: "x = Item rule dot origin endp"
-      "rule \<in> set \<RR>" "dot \<le> length (item_rule_body x)" "origin \<le> length inp" "endp \<le> length inp"
+      "rule \<in> set (\<RR> cfg)" "dot \<le> length (item_rule_body x)" "origin \<le> length inp" "endp \<le> length inp"
       unfolding wf_item_def using item.exhaust_sel le_trans by blast
-    hence "length (rule_body rule) \<in> { length (rule_body r) | r. r \<in> set \<RR> }"
+    hence "length (rule_body rule) \<in> { length (rule_body r) | r. r \<in> set (\<RR> cfg) }"
       using *(1,2) item_rule_body_def by blast
-    moreover have "finite { length (rule_body r) | r. r \<in> set \<RR> }"
-      using finite finite_image_set[of "\<lambda>x. x \<in> set \<RR>"] by fastforce
+    moreover have "finite { length (rule_body r) | r. r \<in> set (\<RR> cfg) }"
+      using finite finite_image_set[of "\<lambda>x. x \<in> set (\<RR> cfg)"] by fastforce
     ultimately have "M \<ge> length (rule_body rule)"
       unfolding M_def by simp
     hence "dot \<le> M"
@@ -1093,13 +1087,11 @@ proof -
 qed
 
 lemma finiteness_UNIV_wf_item:
-  "finite { x | x. wf_item \<RR> inp x }"
+  "finite { x | x. wf_item cfg inp x }"
   using finiteness_empty finiteness_nonempty by fastforce
 
 theorem finiteness:
-  "finite (\<II> inp)"
+  "finite (\<II> cfg inp)"
   using finiteness_UNIV_wf_item wf_items_def wf_\<II> rev_finite_subset by (metis mem_Collect_eq subsetI)
-
-end
 
 end
